RISC-V: exception case (WIP)

case_study/RiscvPmp/Contracts.v
@@ -104,23 +104,6 @@ Module RiscvPmpSymbolicContractKit <: (SymbolicContractKit RiscvPmpTermKit
                                   RiscvPmpProgramKit
                                   RiscvPmpAssertionKit.
 
-  Local Notation "'rs'"      := "rs" : string_scope.
-  Local Notation "'rs1'"     := "rs1" : string_scope.
-  Local Notation "'rs2'"     := "rs2" : string_scope.
-  Local Notation "'rd'"      := "rd" : string_scope.
-  Local Notation "'op'"      := "op" : string_scope.
-  Local Notation "'v'"       := "v" : string_scope.
-  Local Notation "'w'"       := "w" : string_scope.
-  Local Notation "'imm'"     := "imm" : string_scope.
-  Local Notation "'t'"       := "t" : string_scope.
-  Local Notation "'addr'"    := "addr" : string_scope.
-  Local Notation "'paddr'"   := "paddr" : string_scope.
-  Local Notation "'typ'"     := "typ" : string_scope.
-  Local Notation "'acc'"     := "acc" : string_scope.
-  Local Notation "'value'"   := "value" : string_scope.
-  Local Notation "'data'"    := "data" : string_scope.
-  Local Notation "'bv'"      := "bv" : string_scope.
-
   Local Notation "r '↦' val" := (asn_chunk (chunk_ptsreg r val)) (at level 100).
   Local Notation "r '↦r' val" := (asn_chunk (chunk_user ptsreg (env_nil ► (ty_regidx ↦ r) ► (ty_xlenbits ↦ val)))) (at level 100).
   Local Notation "p '∗' q" := (asn_sep p q) (at level 150).
@@ -167,7 +150,7 @@ Module RiscvPmpSymbolicContractKit <: (SymbolicContractKit RiscvPmpTermKit
   (* ∀ r : regidx, ∃ w : xlenbits, r ↦r w *)
   Definition asn_regs_ptsto {Σ} : Assertion Σ :=
     asn_and_regs
-      (fun r => asn_exist w ty_xlenbits (term_lit ty_regidx r ↦r term_var w)).
+      (fun r => asn_exist "w" ty_xlenbits (term_lit ty_regidx r ↦r term_var "w")).
 
   (* TODO: abstract away the concrete type, look into unions for that *)
   (* TODO: length of list should be 16, no duplicates *)
@@ -175,6 +158,9 @@ Module RiscvPmpSymbolicContractKit <: (SymbolicContractKit RiscvPmpTermKit
     term_list (cons (term_binop binop_pair
                                 (term_lit ty_pmpcfgidx PMP0CFG) (* PMP0CFG ↦ ... *)
                                 (term_lit ty_pmpaddridx PMPADDR0)) nil). (* PMPADDR0 ↦ ... *)
+
+  Section Contracts.
+    Import RiscvNotations.
 
   (** Machine Invariant **)
   (*
@@ -202,6 +188,8 @@ Module RiscvPmpSymbolicContractKit <: (SymbolicContractKit RiscvPmpTermKit
        sep_contract_postcondition   :=
          asn_pmp_entries (term_var "entries") ∗
          asn_regs_ptsto ∗
+         mtvec ↦ (term_var "h") ∗
+         asn_exist v ty_xlenbits (nextpc ↦ term_var v) ∗
          asn_or (cur_privilege ↦ (term_var "m") ∗ pc ↦ (term_var "i"))
                 (cur_privilege ↦ (term_lit ty_privilege Machine) ∗
                  pc ↦ (term_var "h") ∗
@@ -226,6 +214,36 @@ Module RiscvPmpSymbolicContractKit <: (SymbolicContractKit RiscvPmpTermKit
 
   Definition sep_contract_execute_RISCV_JALR : SepContractFun execute_RISCV_JALR :=
     mach_inv_contract.
+
+  Definition sep_contract_execute_ECALL : SepContractFun execute_ECALL :=
+    mach_inv_contract.
+
+  Definition sep_contract_exception_handler : SepContractFun exception_handler :=
+    {| sep_contract_logic_variables := [cur_priv ∶ ty_privilege, ctl ∶ ty_ctl_result, "pc" ∶ ty_xlenbits];
+       sep_contract_localstore      := [term_var cur_priv, term_var ctl, term_var "pc"]%arg;
+       sep_contract_precondition    := asn_true;
+       sep_contract_result          := "result_exception_handler";
+       sep_contract_postcondition   := asn_true;
+    |}.
+
+  Definition sep_contract_prepare_trap_vector : SepContractFun prepare_trap_vector :=
+    {| sep_contract_logic_variables := [p ∶ ty_privilege, cause ∶ ty_mcause, tvec ∶ ty_xlenbits];
+       sep_contract_localstore      := [term_var p, term_var cause]%arg;
+       sep_contract_precondition    := mtvec ↦ (term_var tvec);
+       sep_contract_result          := "result_prepare_trap_vector";
+       sep_contract_postcondition   :=
+         asn_eq (term_var "result_prepare_trap_vector") (term_var tvec)
+         ∗ mtvec ↦ (term_var tvec);
+    |}.
+
+  Definition sep_contract_tvec_addr : SepContractFun tvec_addr :=
+    {| sep_contract_logic_variables := [m ∶ ty_xlenbits, c ∶ ty_mcause];
+       sep_contract_localstore      := [term_var m, term_var c]%arg;
+       sep_contract_precondition    := asn_true;
+       sep_contract_result          := "result_tvec_addr";
+       sep_contract_postcondition   :=
+         asn_eq (term_var "result_tvec_addr") (term_inl (term_var m));
+    |}.
 
   Definition sep_contract_get_arch_pc : SepContractFun get_arch_pc :=
     {| sep_contract_logic_variables := [v ∶ ty_xlenbits];
@@ -264,17 +282,17 @@ Module RiscvPmpSymbolicContractKit <: (SymbolicContractKit RiscvPmpTermKit
          asn_match_enum
            regidx (term_var rs)
            (fun k => match k with
-                     | X0 => asn_true
+                     | X0 => asn_eq (term_var v) (term_lit ty_int 0%Z)
                      | _  => term_var rs ↦r term_var v
                      end);
        sep_contract_result          := "result_rX";
        sep_contract_postcondition   :=
-         asn_match_enum
+         asn_eq (term_var "result_rX") (term_var v)
+         ∗ asn_match_enum
            regidx (term_var rs)
            (fun k => match k with
-                     | X0 => asn_eq (term_var "result_rX") (term_lit ty_int 0%Z)
-                     | _  => asn_eq (term_var "result_rX") (term_var v)
-                             ∗ term_var rs ↦r term_var v 
+                     | X0 => asn_true
+                     | _  => term_var rs ↦r term_var v
                      end)
     |}.
 
@@ -352,22 +370,28 @@ Module RiscvPmpSymbolicContractKit <: (SymbolicContractKit RiscvPmpTermKit
        lemma_postcondition   := term_enum regidx r ↦r term_var w
     |}.
 
+  End Contracts.
+
   Definition CEnv : SepContractEnv :=
     fun Δ τ f =>
       match f with
-      | execute_RTYPE      => Some sep_contract_execute_RTYPE
-      | execute_ITYPE      => Some sep_contract_execute_ITYPE
-      | execute_UTYPE      => Some sep_contract_execute_UTYPE
-      | execute_BTYPE      => Some sep_contract_execute_BTYPE
-      | execute_RISCV_JAL  => Some sep_contract_execute_RISCV_JAL
-      | execute_RISCV_JALR => Some sep_contract_execute_RISCV_JALR
-      | get_arch_pc        => Some sep_contract_get_arch_pc
-      | get_next_pc        => Some sep_contract_get_next_pc
-      | set_next_pc        => Some sep_contract_set_next_pc
-      | rX                 => Some sep_contract_rX
-      | wX                 => Some sep_contract_wX
-      | abs                => Some sep_contract_abs
-      | _                  => None
+      | execute_RTYPE       => Some sep_contract_execute_RTYPE
+      | execute_ITYPE       => Some sep_contract_execute_ITYPE
+      | execute_UTYPE       => Some sep_contract_execute_UTYPE
+      | execute_BTYPE       => Some sep_contract_execute_BTYPE
+      | execute_RISCV_JAL   => Some sep_contract_execute_RISCV_JAL
+      | execute_RISCV_JALR  => Some sep_contract_execute_RISCV_JALR
+      | execute_ECALL       => Some sep_contract_execute_ECALL
+      | get_arch_pc         => Some sep_contract_get_arch_pc
+      | get_next_pc         => Some sep_contract_get_next_pc
+      | set_next_pc         => Some sep_contract_set_next_pc
+      | exception_handler   => Some sep_contract_exception_handler
+      | prepare_trap_vector => Some sep_contract_prepare_trap_vector
+      | tvec_addr           => Some sep_contract_tvec_addr
+      | rX                  => Some sep_contract_rX
+      | wX                  => Some sep_contract_wX
+      | abs                 => Some sep_contract_abs
+      | _                   => None
       end.
 
   Definition CEnvEx : SepContractEnvEx :=
@@ -417,6 +441,12 @@ Definition ValidContractDebug {Δ τ} (f : Fun Δ τ) : Prop :=
   | None => False
   end.
 
+Lemma valid_contract_prepare_trap_vector : ValidContract prepare_trap_vector.
+Proof. reflexivity. Qed.
+
+Lemma valid_contract_tvec_addr : ValidContract tvec_addr.
+Proof. reflexivity. Qed.
+
 Lemma valid_contract_get_arch_pc : ValidContract get_arch_pc.
 Proof. reflexivity. Qed.
 
@@ -435,34 +465,55 @@ Proof. reflexivity. Qed.
 Lemma valid_contract_abs : ValidContract abs.
 Proof. reflexivity. Qed.
 
-Lemma valid_contract_execute_RTYPE : ValidContractDebug execute_RTYPE.
-Proof. compute; firstorder. Qed.
-Lemma valid_contract_execute_RTYPE' : ValidContract execute_RTYPE.
-Proof. Admitted. (* reflexivity. Qed. *)
+Lemma valid_contract_execute_RTYPE : ValidContract execute_RTYPE.
+Proof. reflexivity. Qed. 
 
-Lemma valid_contract_execute_ITYPE : ValidContractDebug execute_ITYPE.
-Proof. compute; firstorder. Qed.
+Lemma valid_contract_execute_ITYPE : ValidContract execute_ITYPE.
+Proof. reflexivity. Qed.
 
-Lemma valid_contract_execute_UTYPE : ValidContractDebug execute_UTYPE.
-Proof. compute; firstorder. Qed.
+Lemma valid_contract_execute_UTYPE : ValidContract execute_UTYPE.
+Proof. reflexivity. Qed.
 
-Lemma valid_contract_execute_BTYPE : ValidContractDebug execute_BTYPE.
-Proof. compute; firstorder. Qed.
+Lemma valid_contract_execute_BTYPE : ValidContract execute_BTYPE.
+Proof. reflexivity. Qed.
 
-Lemma valid_contract_execute_RISCV_JAL : ValidContractDebug execute_RISCV_JAL.
-Proof. compute; firstorder. Qed.
+Lemma valid_contract_execute_RISCV_JAL : ValidContract execute_RISCV_JAL.
+Proof. reflexivity. Qed.
 
-Lemma valid_contract_execute_RISCV_JALR : ValidContractDebug execute_RISCV_JALR.
-Proof. compute; firstorder. Qed.
+Lemma valid_contract_execute_RISCV_JALR : ValidContract execute_RISCV_JALR.
+Proof. reflexivity. Qed.
+
+Section Debug.
+  Import RiscvNotations.
+  Import RiscvμSailNotations.
+  Coercion stm_exp : Exp >-> Stm.
+
+  Definition fun_execute_ECALL' : Stm ctx_nil ty_retired :=
+    let: tmp1 := stm_read_register cur_privilege in
+    let: t := match: tmp1 in privilege with
+              | Machine => E_M_EnvCall
+              | User    => E_U_EnvCall
+              end in
+    let: tmp2 := stm_read_register pc in
+    let: tmp3 := stm_debugk (call exception_handler tmp1 (CTL_TRAP t) tmp2) in
+    call set_next_pc tmp3 ;;
+    stm_lit ty_retired RETIRE_FAIL.
+
+  Lemma valid_contract_execute_ECALL : SMut.ValidContract sep_contract_execute_ECALL fun_execute_ECALL'.
+  Proof.
+    compute.
+  Admitted.
+  (* firstorder. Qed. *)
+End Debug.
 
 (* TODO: this is just to make sure that all contracts defined so far are valid
          (i.e. ensure no contract was defined and then forgotten to validate it) *)
 Lemma defined_contracts_valid : forall {Δ τ} (f : Fun Δ τ),
     match CEnv f with
-    | Some c => ValidContract f \/ ValidContractDebug f
+    | Some c => ValidContract f
     | None => True
     end.
 Proof.
   destruct f; simpl; trivial;
-    (left; reflexivity) || (right; compute; firstorder).
-Qed.
+    try reflexivity.
+Admitted.
